stlc with subtyping (nano4)

dev2015/nano4.v
@@ -1,6 +1,7 @@
 (* Full safety for STLC *)
 (* values well-typed with respect to runtime environment *)
 (* inversion lemma structure *)
+(* subtyping (in addition to nano2.v) *)
 
 Require Export SfLib.
 
@@ -12,8 +13,10 @@ Module STLC.
 Definition id := nat.
 
 Inductive ty : Type :=
-  | TBool  : ty
+  | TBool  : ty           
   | TFun   : ty -> ty -> ty
+  | TBot   : ty
+  | TTop   : ty
 .
 
 Inductive tm : Type :=
@@ -25,8 +28,8 @@ Inductive tm : Type :=
 .
 
 Inductive vl : Type :=
-| vbool : bool -> vl
-| vabs  : list vl -> tm -> vl
+  | vbool : bool -> vl
+  | vabs  : list vl -> tm -> vl
 .
 
 Definition venv := list vl.
@@ -35,12 +38,6 @@ Definition tenv := list ty.
 Hint Unfold venv.
 Hint Unfold tenv.
 
-Fixpoint length {X: Type} (l : list X): nat :=
-  match l with
-    | [] => 0
-    | _::l' => 1 + length l'
-  end.
-
 Fixpoint index {X : Type} (n : id) (l : list X) : option X :=
   match l with
     | [] => None
@@ -48,42 +45,142 @@ Fixpoint index {X : Type} (n : id) (l : list X) : option X :=
   end.
 
 
-Inductive has_type : tenv -> tm -> ty -> Prop :=
-| t_true: forall env,
-           has_type env ttrue TBool
-| t_false: forall env,
-           has_type env tfalse TBool
-| t_var: forall x env T1,
-           index x env = Some T1 ->
-           has_type env (tvar x) T1
-| t_app: forall env f x T1 T2,
-           has_type env f (TFun T1 T2) ->
-           has_type env x T1 ->
-           has_type env (tapp f x) T2
-| t_abs: forall env y T1 T2,
-           has_type (T1::(TFun T1 T2)::env) y T2 -> 
-           has_type env (tabs y) (TFun T1 T2)
+Inductive closed: nat -> ty -> Prop :=
+| cl_bot: forall k,
+    closed k TBot
+| cl_top: forall k,
+    closed k TTop
+| cl_bool: forall k,
+    closed k TBool
+| cl_fun: forall k T1 T2,
+    closed k T1 ->
+    closed k T2 ->
+    closed k (TFun T1 T2)
 .
 
-Inductive wf_env : venv -> tenv -> Prop := 
+Inductive stp: tenv -> ty -> ty -> Prop :=
+| stp_bot: forall G1 T1,
+    closed (length G1) T1 ->
+    stp G1 TBot T1
+| stp_top: forall G1 T1,
+    closed (length G1) T1 ->
+    stp G1 T1 TTop
+| stp_bool: forall G1,
+    stp G1 TBool TBool
+| stp_fun: forall G1 T1 T2 T3 T4,
+    stp G1 T3 T1 ->
+    stp G1 T2 T4 ->
+    stp G1 (TFun T1 T2) (TFun T3 T4)
+.
+
+
+Inductive has_type : tenv -> tm -> ty -> Prop :=
+| t_true: forall env,
+    has_type env ttrue TBool
+| t_false: forall env,
+    has_type env tfalse TBool
+| t_var: forall x env T1,
+    index x env = Some T1 ->
+    has_type env (tvar x) T1
+| t_app: forall env f x T1 T2,
+    has_type env f (TFun T1 T2) ->
+    has_type env x T1 ->
+    has_type env (tapp f x) T2
+| t_abs: forall env y T1 T2,
+    has_type (T1::(TFun T1 T2)::env) y T2 ->
+    closed (length env) (TFun T1 T2) ->       
+    has_type env (tabs y) (TFun T1 T2)
+| t_sub: forall env x T1 T2,
+    has_type env x T1 ->
+    stp env T1 T2 ->
+    has_type env x T2
+.
+
+Inductive stp2: bool -> venv -> ty -> venv -> ty -> nat -> Prop :=
+| stp2_bot: forall G1 G2 T n1,
+    closed (length G2) T ->
+    stp2 true G1 TBot G2 T (S n1)
+| stp2_top: forall G1 G2 T n1,
+    closed (length G1) T ->
+    stp2 true G1 T G2 TTop (S n1)
+| stp2_bool: forall G1 G2 n1,
+    stp2 true G1 TBool G2 TBool (S n1)
+| stp2_fun: forall G1 G2 T1 T2 T3 T4 n1 n2,
+    stp2 false G2 T3 G1 T1 n1 ->
+    stp2 false G1 T2 G2 T4 n2 ->
+    stp2 true G1 (TFun T1 T2) G2 (TFun T3 T4) (S (n1+n2))
+| stp2_wrapf: forall G1 G2 T1 T2 n1,
+    stp2 true G1 T1 G2 T2 n1 ->
+    stp2 false G1 T1 G2 T2 (S n1)
+| stp2_transf: forall G1 G2 G3 T1 T2 T3 n1 n2,
+    stp2 true G1 T1 G2 T2 n1 ->
+    stp2 false G2 T2 G3 T3 n2 ->
+    stp2 false G1 T1 G3 T3 (S (n1+n2))
+         
+
+with wf_env : venv -> tenv -> Prop := 
 | wfe_nil : wf_env nil nil
 | wfe_cons : forall v t vs ts,
     val_type (v::vs) v t ->
     wf_env vs ts ->
     wf_env (cons v vs) (cons t ts)
 
-with val_type : venv -> vl -> ty -> Prop :=
-| v_bool: forall venv b,
-    val_type venv (vbool b) TBool
-| v_abs: forall env venv tenv y T1 T2,
+with val_type0 : venv -> vl -> ty -> Prop :=
+| v_bool: forall b,
+    val_type0 [] (vbool b) TBool
+| v_abs: forall venv tenv y T1 T2,
     wf_env venv tenv ->
     has_type (T1::(TFun T1 T2)::tenv) y T2 ->
-    val_type env (vabs venv y) (TFun T1 T2)
+    val_type0 venv (vabs venv y) (TFun T1 T2)
+              
+with val_type : venv -> vl -> ty -> Prop :=
+| v_sub: forall G1 T1 G2 T2 v,
+    val_type0 G1 v T1 ->
+    (exists n, stp2 true G1 T1 G2 T2 n) ->
+    val_type G2 v T2
 .
+              
 
-Inductive stp: venv -> ty -> venv -> ty -> Prop :=
-| stp_refl: forall G1 G2 T,
-   stp G1 T G2 T.
+
+Definition stpd2 m G1 T1 G2 T2 := exists n, stp2 m G1 T1 G2 T2 n.
+
+Hint Constructors stp2.
+
+Ltac ep := match goal with
+             | [ |- stp2 ?M ?G1 ?T1 ?G2 ?T2 ?N ] => assert (exists (n:nat), stp2 M G1 T1 G2 T2 n) as EEX
+           end.
+
+Ltac eu := match goal with
+             | H: stpd2 _ _ _ _ _ |- _ => destruct H as [? H]
+           end.
+
+Lemma stpd2_bot: forall G1 G2 T,
+    closed (length G2) T ->
+    stpd2 true G1 TBot G2 T.
+Proof. intros. exists 1. eauto. Qed.
+Lemma stpd2_top: forall G1 G2 T,
+    closed (length G1) T ->
+    stpd2 true G1 T G2 TTop.
+Proof. intros. exists 1. eauto. Qed.
+Lemma stpd2_bool: forall G1 G2,
+    stpd2 true G1 TBool G2 TBool.
+Proof. intros. exists 1. eauto. Qed.
+Lemma stpd2_fun: forall G1 G2 T1 T2 T3 T4,
+    stpd2 false G2 T3 G1 T1 ->
+    stpd2 false G1 T2 G2 T4 ->
+    stpd2 true  G1 (TFun T1 T2) G2 (TFun T3 T4).
+Proof. intros. repeat eu. eexists. eauto. Qed.
+
+Lemma stpd2_wrapf: forall G1 G2 T1 T2,
+    stpd2 true G1 T1 G2 T2 ->
+    stpd2 false G1 T1 G2 T2.
+Proof. intros. repeat eu. eexists. eauto. Qed.
+Lemma stpd2_transf: forall G1 G2 G3 T1 T2 T3,
+    stpd2 true G1 T1 G2 T2 ->
+    stpd2 false G2 T2 G3 T3 ->
+    stpd2 false G1 T1 G3 T3.
+Proof. intros. repeat eu. eexists. eauto. Qed.
+
 
 
 
@@ -93,7 +190,7 @@ Some None        means stuck
 Some (Some v))   means result v
 
 Could use do-notation to clean up syntax.
- *)
+*)
 
 Fixpoint teval(n: nat)(env: venv)(t: tm){struct n}: option (option vl) :=
   match n with
@@ -127,8 +224,11 @@ Hint Constructors vl.
 
 
 Hint Constructors has_type.
+Hint Constructors stp2.
 Hint Constructors val_type.
 Hint Constructors wf_env.
+
+Hint Unfold stpd2.
 
 Hint Constructors option.
 Hint Constructors list.
@@ -137,6 +237,16 @@ Hint Unfold index.
 Hint Unfold length.
 
 Hint Resolve ex_intro.
+
+
+Ltac ev := repeat match goal with
+                    | H: exists _, _ |- _ => destruct H
+                    | H: _ /\  _ |- _ => destruct H
+           end.
+
+
+
+
 
 Lemma wf_length : forall vs ts,
                     wf_env vs ts ->
@@ -169,10 +279,22 @@ Proof.
   compute. eauto.
 Qed.
 
-Lemma valtp_extend : forall vs v v1 T,
-                       val_type vs v T ->
-                       val_type (v1::vs) v T.
-Proof. intros. induction H; eauto. Qed.
+Lemma index_exists : forall X vs n,
+                       n < length vs ->
+                       exists (T:X), index n vs = Some T.
+Proof.
+  intros X vs. induction vs.
+  Case "nil". intros. inversion H.
+  Case "cons".
+  intros. inversion H.
+  SCase "hit".
+  assert (beq_nat n (length vs) = true) as E. eapply beq_nat_true_iff. eauto.
+  simpl. subst n. rewrite E. eauto.
+  SCase "miss".
+  assert (beq_nat n (length vs) = false) as E. eapply beq_nat_false_iff. omega.
+  simpl. rewrite E. eapply IHvs. eauto.
+Qed.
+
 
 Lemma index_extend : forall X vs n a (T: X),
                        index n vs = Some T ->
@@ -185,6 +307,97 @@ Proof.
   assert (beq_nat n (length vs) = false) as E. eapply beq_nat_false_iff; eauto.
   unfold index. unfold index in H. rewrite H. rewrite E. reflexivity.
 Qed.
+
+
+Lemma closed_extend : forall X (a:X) G T,
+                       closed (length G) T ->
+                       closed (length (a::G)) T.
+Proof.
+  intros. induction T; inversion H;  econstructor; eauto.
+Qed.
+
+
+Lemma stp2_extend : forall m v1 G1 G2 T1 T2 n,
+                      stp2 m G1 T1 G2 T2 n ->
+                      stp2 m (v1::G1) T1 G2 T2 n /\
+                      stp2 m G1 T1 (v1::G2) T2 n /\
+                      stp2 m (v1::G1) T1 (v1::G2) T2 n.
+Proof.
+  intros. induction H; try solve [repeat split; econstructor; try eauto;
+          try eapply IHstp2; eauto;
+          try eapply index_extend; eauto; try eapply closed_extend; eauto;
+          try eapply IHstp2_1; try eapply IHstp2_2;
+            try eapply IHstp2_3; try eapply IHstp2_4].
+
+  (* trans case left *)
+  
+  repeat split; eapply stp2_transf; try eapply IHstp2_1; eauto; try eapply IHstp2_2; eauto.
+Qed.
+
+Lemma stpd2_extend : forall m v1 G1 G2 T1 T2,
+                      stpd2 m G1 T1 G2 T2 ->
+                      stpd2 m (v1::G1) T1 G2 T2 /\
+                      stpd2 m G1 T1 (v1::G2) T2 /\
+                      stpd2 m (v1::G1) T1 (v1::G2) T2.
+Proof.
+  intros. repeat eu. repeat split; eexists; eapply stp2_extend; eauto.
+Qed.
+
+
+Lemma stp2_extend1 : forall m v1 G1 G2 T1 T2 n, stp2 m G1 T1 G2 T2 n -> stp2 m (v1::G1) T1 G2 T2 n.
+Proof. intros. eapply stp2_extend. eauto. Qed.
+
+Lemma stp2_extend2 : forall m v1 G1 G2 T1 T2 n, stp2 m G1 T1 G2 T2 n -> stp2 m G1 T1 (v1::G2) T2 n.
+Proof. intros. eapply stp2_extend. eauto. Qed.
+
+Lemma stpd2_extend1 : forall m v1 G1 G2 T1 T2, stpd2 m G1 T1 G2 T2 -> stpd2 m (v1::G1) T1 G2 T2.
+Proof. intros. eapply stpd2_extend. eauto. Qed.
+
+Lemma stpd2_extend2 : forall m v1 G1 G2 T1 T2, stpd2 m G1 T1 G2 T2 -> stpd2 m G1 T1 (v1::G2) T2.
+Proof. intros. eapply stpd2_extend. eauto. Qed.
+
+
+
+Lemma stp_closed : forall G1 T1 T2,
+                      stp G1 T1 T2 ->
+                      closed (length G1) T1 /\
+                      closed (length G1) T2.
+Proof.
+  intros. induction H; repeat split; try  econstructor; try eapply IHstp1; try eapply IHstp2; eauto; try eapply IHstp; eauto; try eapply index_max; eauto.
+  (* destruct IHstp. inversion H1. eauto.
+  destruct IHstp2. inversion H3. eauto. *)
+Qed.
+
+
+
+Lemma stpd2_closed : forall m G1 G2 T1 T2,
+                      stpd2 m G1 T1 G2 T2 ->
+                      closed (length G1) T1 /\
+                      closed (length G2) T2.
+Proof.
+  intros. eu. induction H; repeat split; try  econstructor; try eapply IHstp2_1; try eapply IHstp2_2; eauto; try eapply IHstp2; eauto; try eapply index_max; eauto.
+  (* destruct IHstp2. inversion H1. eauto.
+  eapply IHstp2_4. *)
+Qed.
+
+Lemma stpd2_closed1 : forall m G1 G2 T1 T2,
+                      stpd2 m G1 T1 G2 T2 ->
+                      closed (length G1) T1.
+Proof. intros. eapply (stpd2_closed m G1 G2); eauto. Qed.
+
+Lemma stpd2_closed2 : forall m G1 G2 T1 T2,
+                      stpd2 m G1 T1 G2 T2 ->
+                      closed (length G2) T2.
+Proof. intros. eapply (stpd2_closed m G1 G2); eauto. Qed.
+
+
+Lemma valtp_extend : forall vs v v1 T,
+                       val_type vs v T ->
+                       val_type (v1::vs) v T.
+Proof.
+  intros. induction H; econstructor; eauto; try eapply stpd2_extend; eauto; try eapply index_extend; eauto. 
+Qed.
+
 
 
 Lemma index_safe_ex: forall H1 G1 TF i,
@@ -220,25 +433,146 @@ Hint Constructors res_type.
 Hint Resolve not_stuck.
 
 
-Lemma valtp_widen: forall vf H1 H2 T1 T2,
-  val_type H1 vf T1 ->
-  stp H1 T1 H2 T2 ->
-  val_type H2 vf T2.
+Lemma stpd2_refl: forall G1 T1,
+  closed (length G1) T1 ->
+  stpd2 true G1 T1 G1 T1.
 Proof.
-  intros. inversion H; inversion H0; subst T2; subst; eauto.
+  intros. induction T1; inversion H.
+  - Case "bool". eapply stpd2_bool; eauto.
+  - Case "fun". eapply stpd2_fun; try eapply stpd2_wrapf; eauto.
+  - Case "bot". exists 1. eauto.
+  - Case "top". exists 1. eauto.
 Qed.
 
 
-Lemma invert_abs: forall venv vf vx T1 T2,
+Lemma stpd2_reg1 : forall m G1 G2 T1 T2,
+                      stpd2 m G1 T1 G2 T2 ->
+                      stpd2 true G1 T1 G1 T1.
+Proof.
+  intros. eapply stpd2_refl. eapply (stpd2_closed m G1 G2). eauto.
+Qed.
+
+Lemma stpd2_reg2 : forall m G1 G2 T1 T2,
+                      stpd2 m G1 T1 G2 T2 ->
+                      stpd2 true G2 T2 G2 T2.
+Proof.
+  intros. eapply stpd2_refl. eapply (stpd2_closed m G1 G2). eauto.
+Qed.
+
+
+Lemma stpd2_trans_axiom_aux: forall n, forall G1 G2 G3 T1 T2 T3 n1,
+  stp2 false G1 T1 G2 T2 n1 -> n1 < n ->
+  stpd2 false G2 T2 G3 T3 ->
+  stpd2 false G1 T1 G3 T3.
+Proof.
+  intros n. induction n; intros; try omega; repeat eu; subst; inversion H; subst.
+  - Case "wrapf". eapply stpd2_transf. eexists. eauto. eexists. eauto. 
+  - Case "transf". eapply stpd2_transf. eexists. eauto. eapply IHn. eauto. omega. eexists. eauto.
+Qed.
+
+
+
+Lemma stp2_trans_axiom: forall m G1 G2 G3 T1 T2 T3,
+  stpd2 m G1 T1 G2 T2 -> 
+  stpd2 false G2 T2 G3 T3 ->
+  stpd2 false G1 T1 G3 T3.
+Proof.
+  intros. destruct m; eu; eu; eapply stpd2_trans_axiom_aux; eauto.
+Qed.
+
+
+Lemma stp2_trans: forall n, forall m G1 G2 G3 T1 T2 T3 n1 n2,
+  stp2 m G1 T1 G2 T2 n1 -> 
+  stp2 true G2 T2 G3 T3 n2 ->
+  n1 < n ->
+  stpd2 true G1 T1 G3 T3.
+Proof.
+  intros n. induction n; intros. solve by inversion.
+  inversion H.
+  - Case "bot". eapply stpd2_bot; eauto. eapply stpd2_closed2; eauto.
+  - Case "top". inversion H0; subst; try solve by inversion.
+    + SCase "top". eapply stpd2_top; eauto.
+  - Case "bool". inversion H0; subst; try solve by inversion.
+    + SCase "top". eapply stpd2_top; eauto. econstructor.
+    + SCase "bool". eapply stpd2_bool; eauto.
+  - Case "fun". inversion H0; subst; try solve by inversion.
+    + SCase "top". eapply stpd2_top; eauto. eapply stpd2_closed1; eauto.
+    + SCase "fun". inversion H14. subst. eapply stpd2_fun; eapply stp2_trans_axiom; eauto.
+  - Case "wrapf".
+    subst. eapply IHn. eapply H2. eapply H0. omega.
+  - Case "transf".
+    assert (stpd2 true G4 T4 G3 T3). eapply IHn. eapply H3. eapply H0. omega.
+    eu. subst. eapply IHn. eapply H2. eauto. omega.
+Qed.
+
+Lemma stpd2_trans: forall m G1 G2 G3 T1 T2 T3,
+  stpd2 m G1 T1 G2 T2 ->
+  stpd2 true G2 T2 G3 T3 ->
+  stpd2 true G1 T1 G3 T3.
+Proof.
+  intros. repeat eu. eapply stp2_trans; eauto.
+Qed.
+
+Lemma stp_to_stpd2: forall G1 T1 T2,
+  stp G1 T1 T2 ->
+  forall GX, wf_env GX G1 -> 
+  stpd2 true GX T1 GX T2.
+Proof.
+  intros G1 T1 T2 H. induction H; intros.
+  - Case "bot". eapply stpd2_bot; eauto. rewrite (wf_length GX G1); eauto.
+  - Case "top". eapply stpd2_top; eauto. rewrite (wf_length GX G1); eauto.
+  - Case "bool". eapply stpd2_bool; eauto.
+  - Case "fun".  eapply stpd2_fun; eapply stpd2_wrapf; eauto.
+Qed.
+
+
+Lemma valtp_widen: forall vf H1 H2 T1 T2,
+  val_type H1 vf T1 ->
+  stpd2 true H1 T1 H2 T2 ->
+  val_type H2 vf T2.
+Proof.
+  intros.  inversion H.
+  - econstructor; eauto. eapply stpd2_trans; eauto.
+Qed.
+
+Lemma restp_widen: forall vf H1 H2 T1 T2,
+  res_type H1 vf T1 ->
+  stpd2 true H1 T1 H2 T2 ->
+  res_type H2 vf T2.
+Proof.
+  intros. inversion H. eapply not_stuck. eapply valtp_widen; eauto.
+Qed.
+
+
+Lemma invert_abs1: forall n, forall venv vf T1 T2 GX TX n1,
+  val_type0 GX vf TX -> stp2 true GX TX venv (TFun T1 T2) n1 -> n1 < n ->
+  exists env tenv y T3 T4,
+    vf = (vabs env y) /\ 
+    wf_env env tenv /\
+    has_type (T3::(TFun T3 T4)::tenv) y T4 /\
+    stpd2 true venv T1 env T3 /\
+    stpd2 true env T4 venv T2.
+Proof.
+  intros n. induction n; intros. solve by inversion.
+  inversion H; subst. 
+  - Case "bool". solve by inversion.
+  - Case "fun". subst. inversion H0. subst.
+    eexists. eexists. eexists. eexists. eexists. repeat split; eauto.
+    eapply stpd2_trans. eauto. eapply stpd2_reg2. eauto.
+    eapply stpd2_trans. eauto. eapply stpd2_reg2. eauto.
+Qed.
+
+
+Lemma invert_abs: forall venv vf T1 T2,
   val_type venv vf (TFun T1 T2) ->
   exists env tenv y T3 T4,
     vf = (vabs env y) /\ 
     wf_env env tenv /\
     has_type (T3::(TFun T3 T4)::tenv) y T4 /\
-    stp venv T1 (vx::vf::env) T3 /\
-    stp (vx::vf::env) T4 venv T2.
+    stpd2 true venv T1 env T3 /\
+    stpd2 true env T4 venv T2.
 Proof.
-  intros. inversion H. repeat eexists; repeat eauto.
+  intros. inversion H. ev. eapply invert_abs1; eauto. 
 Qed.
 
 
@@ -251,46 +585,63 @@ Theorem full_safety : forall n e tenv venv res T,
 Proof.
   intros n. induction n.
   (* 0 *)   intros. inversion H.
-  (* S n *) intros. destruct e; inversion H; inversion H0.
+  (* S n *) intros. destruct e; inversion H.
+
+  - Case "True".
+    remember (ttrue) as e. induction H0; inversion Heqe; subst.
+    + eapply not_stuck. eapply v_sub; eauto. eapply v_bool; eauto.
+    + eapply restp_widen. eapply IHhas_type; eauto. eapply stp_to_stpd2; eauto. 
+
+  - Case "False".
+    remember (tfalse) as e. induction H0; inversion Heqe; subst.
+    + eapply not_stuck. eapply v_sub; eauto. eapply v_bool; eauto.
+    + eapply restp_widen. eapply IHhas_type; eauto. eapply stp_to_stpd2; eauto. 
   
-  Case "True".  eapply not_stuck. eapply v_bool.
-  Case "False". eapply not_stuck. eapply v_bool.
+  - Case "Var".
+    remember (tvar i) as e. induction H0; inversion Heqe; subst.
+    + destruct (index_safe_ex venv0 env T1 i) as [v [I V]]; eauto.
+      rewrite I. eapply not_stuck. eauto. 
+    + eapply restp_widen. eapply IHhas_type; eauto. eapply stp_to_stpd2; eauto. 
 
-  Case "Var".
-    destruct (index_safe_ex venv0 tenv0 T i) as [v [I V]]; eauto. 
-
-    rewrite I. eapply not_stuck. eapply V.
-
-  Case "App".
-    remember (teval n venv0 e1) as tf.
-    remember (teval n venv0 e2) as tx. 
-    subst T.
+  - Case "App".
+    remember (tapp e1 e2) as e. induction H0; inversion Heqe; subst.
+    +
+      remember (teval n venv0 e1) as tf.
+      remember (teval n venv0 e2) as tx. 
     
-    destruct tx as [rx|]; try solve by inversion.
-    assert (res_type venv0 rx T1) as HRX. SCase "HRX". subst. eapply IHn; eauto.
-    inversion HRX as [? vx]. 
+      destruct tx as [rx|]; try solve by inversion.
+      assert (res_type venv0 rx T1) as HRX. SCase "HRX". subst. eapply IHn; eauto.
+      inversion HRX as [? vx]. 
 
-    destruct tf as [rf|]; subst rx; try solve by inversion.  
-    assert (res_type venv0 rf (TFun T1 T2)) as HRF. SCase "HRF". subst. eapply IHn; eauto.
-    inversion HRF as [? vf].
+      destruct tf as [rf|]; subst rx; try solve by inversion.  
+      assert (res_type venv0 rf (TFun T1 T2)) as HRF. SCase "HRF". subst. eapply IHn; eauto.
+      inversion HRF as [? vf].
 
-    destruct (invert_abs venv0 vf vx T1 T2) as
-        [env1 [tenv [y0 [T3 [T4 [EF [WF [HTY [STX STY]]]]]]]]]. eauto.
-    (* now we know it's a closure, and we have has_type evidence *)
+      destruct (invert_abs venv0 vf T1 T2) as
+          [env1 [tenv [y0 [T3 [T4 [EF [WF [HTY [STX STY]]]]]]]]]. eauto.
+      (* now we know it's a closure, and we have has_type evidence *)
 
-    assert (res_type (vx::vf::env1) res T4) as HRY.
-      SCase "HRY".
-        subst. eapply IHn. eauto. eauto.
-        (* wf_env f x *) econstructor. eapply valtp_widen; eauto.
-        (* wf_env f   *) econstructor. eapply v_abs; eauto.
-        eauto.
+      assert (res_type (vx::vf::env1) res T4) as HRY.
+        SCase "HRY".
+          subst. eapply IHn. eauto. eauto.
+          (* wf_env f x *) econstructor. eapply valtp_widen; eauto. eapply stpd2_extend2; eauto. eapply stpd2_extend2; eauto.
+          (* wf_env f   *) econstructor. eapply v_sub. eapply v_abs; eauto. eapply stpd2_extend2. eapply stpd2_fun. eapply stpd2_wrapf. eapply stpd2_reg2; eauto. eapply stpd2_wrapf. eapply stpd2_reg1; eauto.
+          eauto.
 
-    inversion HRY as [? vy].
+      inversion HRY as [? vy].
 
-    eapply not_stuck. eapply valtp_widen; eauto.
+      eapply not_stuck. eapply valtp_widen; eauto. eapply stpd2_extend1. eapply stpd2_extend1. eauto.
+
+    + eapply restp_widen. eapply IHhas_type; eauto. eapply stp_to_stpd2; eauto. 
+
     
-  Case "Abs". intros. inversion H. inversion H0.
-    eapply not_stuck. eapply v_abs; eauto.
+  - Case "Abs". 
+    remember (tabs e) as xe. induction H0; inversion Heqxe; subst.
+    + eapply not_stuck. eapply v_sub. eapply v_abs; eauto. eapply stpd2_refl. rewrite (wf_length venv0 env). eauto. eauto. 
+    + eapply restp_widen. eapply IHhas_type; eauto. eapply stp_to_stpd2; eauto. 
+
+Grab Existential Variables.
+apply 0. apply 0. 
 Qed.
 
 End STLC.
